Clase5.Listas.fst
@@ -11,12 +11,16 @@ let rec sum_int xs =
 (* Demuestre que sum_int "distribuye" sobre la concatenación de listas. *)
 let rec sum_append (l1 l2 : list int)
   : Lemma (sum_int (l1 @ l2) == sum_int l1 + sum_int l2)
-  = admit()
+  = match l1 with
+    | [] -> ()
+    | _::xs -> sum_append xs l2
 
 (* Idem para length, definida en la librería de F*. *)
 let rec len_append (l1 l2 : list int)
   : Lemma (length (l1 @ l2) == length l1 + length l2)
-  = admit()
+  = match l1 with
+    | [] -> ()
+    | _::xs -> len_append xs l2
 
 let rec snoc (xs : list int) (x : int) : list int =
   match xs with
@@ -32,14 +36,36 @@ let rec rev_int (xs : list int) : list int =
   | [] -> []
   | x::xs' -> snoc (rev_int xs') x
 
-let rev_append_int (xs ys : list int)
-  : Lemma (rev_int (xs @ ys) == rev_int ys @ rev_int xs)
-= admit()
+let rec snoc_append (xs ys : list int) (z : int)
+  : Lemma (snoc (xs @ ys) z == xs @ snoc ys z)
+= match xs with
+  | [] -> ()
+  | x::xs' -> snoc_append xs' ys z
 
-let rev_rev (xs : list int)
+let rec rev_append_int (xs ys : list int)
+  : Lemma (rev_int (xs @ ys) == rev_int ys @ rev_int xs)
+= match xs with
+  | [] -> ()
+  | x::xs' -> (
+    rev_append_int xs' ys;
+    snoc_append (rev_int ys) (rev_int xs') x
+  )
+
+let rec snoc_cons (l: list int) (z: int)
+  : Lemma (rev_int (snoc l z) == z :: rev_int l)
+= match l with
+  | [] -> ()
+  | h::tl -> snoc_cons tl z
+
+let rec rev_rev (xs : list int)
   : Lemma (rev_int (rev_int xs) == xs)
-= admit()
+= match xs with
+  | [] -> ()
+  | x::xs' -> (
+    rev_rev xs';
+    snoc_cons (rev_int xs') x
+  )
 
 let rev_injective (xs ys : list int)
   : Lemma (requires rev_int xs == rev_int ys) (ensures xs == ys)
-= admit()
+= rev_rev xs; rev_rev ys
